separate extraction and large elim

theories/extraction/ExtractionSort.v
@@ -1,60 +1,20 @@
+Require Import LargeElim.
+
 Sort Info Erase.
 
 Constraint Info ~> Erase, Info ~> Type, Erase ~> Type.
 
 Set Universe Polymorphism.
 
-Class LargeElimSort@{s;l|Type~>s} : Type@{l+2} :=
-{ Univ : 𝒰@{s;l+1} ;
-  code : 𝒰@{s;l} -> Univ ;   
-  El : Univ -> 𝒰@{s;l} ;
-  El_code A : El (code A) = A :> 𝒰@{s;l} }.
-
-Instance TypeLargeElimSort@{l} : LargeElimSort@{Type;l} := {
-    Univ := Type@{l} ; code := fun A => A ; El := fun A => A ; El_code := fun A => eq_refl}.
-
-Definition lift_El@{s;l |Type~>s} {H:LargeElimSort@{s;l}} (A:𝒰@{s;l}) : A -> H.(El) (H.(code) A) :=
-  fun a => eq_poly _ (fun X => X) a _ (eq_sym (H.(El_code) A)).
-
-Definition unlift_El@{s;l |Type~>s} {H:LargeElimSort@{s;l}} (A:𝒰@{s;l}) : H.(El) (H.(code) A) -> A :=
-  fun a => eq_poly _ (fun X => X) a _ (H.(El_code) _).
-
-
-Inductive nat : 𝒰 :=
-  | O : nat
-  | S : nat -> nat.
-
-Inductive unit : 𝒰 := tt.
-Inductive empty : 𝒰 := .
-
-Definition nat_rect@{i} := nat_poly@{Type Type; i}.
-Definition nat_rec@{} := nat_poly@{Type Type; 0}.
-Definition nat_ind@{} := nat_poly@{Type Prop; 0}.
-Definition nat_sind@{} := nat_poly@{Type SProp; 0}.
-
-(*
-Definition P {H:LargeElimSort} (n : nat) :=
-  match n return H.(Univ) with
-    O => code unit
-  | _ => code empty
-  end.
-
-Lemma eq_true {H:LargeElimSort} : forall (n:nat), O = n -> H.(El) (P n).
+Lemma nat_discr_info (n : nat@{Info;}): O = S n -> False.
 Proof.
-  intros b e. destruct e. exact (lift_El _ tt).
+  apply (nat_discr n).
 Qed.
 
-Lemma nat_discr_gen {H:LargeElimSort} (n : nat): O = S n -> empty.
+Lemma nat_discr_erase (n : nat@{Erase;}): O = S n -> False.
 Proof.
-  intro e. exact (unlift_El _ (eq_true _ e)).
+  apply (nat_discr n).
 Qed.
-
-
-Lemma nat_discr (n : nat@{Info;}): O = S n -> False.
-Proof.
-  intro e. pose proof (nat_discr_gen n e). destruct X.
-Qed.
-*)
 
 Inductive Vect (A : 𝒰@{Info;_}) : nat@{Erase;} -> 𝒰@{Info;_} :=
 | vnil : Vect A O
