theories/Init/LargeElim.v
@@ -1,0 +1,66 @@
+Require Import Notations.
+Require Import Ltac.
+Require Import Logic.
+
+Set Universe Polymorphism.
+
+Class LargeElimSort@{s;l|Type~>s} : Type@{l+2} :=
+{ Univ : 𝒰@{s;l+1} ;
+  code : 𝒰@{s;l} -> Univ ;
+  El : Univ -> 𝒰@{s;l} ;
+  El_code A : El (code A) = A :> 𝒰@{s;l} }.
+
+Instance TypeLargeElimSort@{l} : LargeElimSort@{Type;l} := {
+    Univ := Type@{l} ; code := fun A => A ; El := fun A => A ; El_code := fun A => eq_refl}.
+
+Definition lift_El@{s;l |Type~>s} {H:LargeElimSort@{s;l}} (A:𝒰@{s;l}) : A -> H.(El) (H.(code) A) :=
+  fun a => eq_poly _ (fun X => X) a _ (eq_sym (H.(El_code) A)).
+
+Definition unlift_El@{s;l |Type~>s} {H:LargeElimSort@{s;l}} (A:𝒰@{s;l}) : H.(El) (H.(code) A) -> A :=
+  fun a => eq_poly _ (fun X => X) a _ (H.(El_code) _).
+
+(* Example of Large Elimination on natural numbers *)
+
+Inductive nat : 𝒰 :=
+  | O : nat
+  | S : nat -> nat.
+
+Inductive unit : 𝒰 := tt.
+Inductive empty : 𝒰 := .
+
+Definition nat_rect@{i} := nat_poly@{Type Type; i}.
+Definition nat_rec@{} := nat_poly@{Type Type; 0}.
+Definition nat_ind@{} := nat_poly@{Type Prop; 0}.
+Definition nat_sind@{} := nat_poly@{Type SProp; 0}.
+
+
+Definition P@{s;l |Type~>s} {H:LargeElimSort@{s;l}} (n : nat@{s;}) :=
+  match n return H.(Univ) with
+    O => code unit
+  | _ => code empty
+  end.
+
+Lemma eq_true@{s;l |Type~>s} {H:LargeElimSort@{s;l}} : forall (n:nat), O = n -> H.(El) (P n).
+Proof.
+  intros b e. destruct e. exact (lift_El _ tt).
+Qed.
+
+Lemma nat_discr_gen@{s;l |Type~>s} {H:LargeElimSort@{s;l}} (n : nat@{s;}) : O = S n -> empty@{s;0_}.
+Proof.
+  intro e. exact (unlift_El _ (eq_true _ e)).
+Qed.
+
+(* Direct Large Elimination *)
+
+Definition Pred_nat@{s ; | s ~> Type} (n : nat@{s;}) :=
+  match n return Type with | O => unit | _ => empty end.
+
+Lemma eq_true'@{s ; | s ~> Type} : forall (n:nat), O = n -> Pred_nat@{s ; } n.
+Proof.
+  intros b e. destruct e. exact tt.
+Qed.
+
+Lemma nat_discr@{s ; | s ~> Type} (n : nat@{s;}) : O = S n -> False.
+Proof.
+  intro e. destruct (eq_true' _ e).
+Qed.
